theories/examples_wf.v
@@ -1,0 +1,367 @@
+From iris.proofmode Require Import proofmode.
+From ltl Require Import ltl_wf.
+
+Section examples.
+  Context {S L : Type}.
+  Context {Rel : S → L → S → Prop}.
+
+  Notation ltl_prop := (ltl_prop S L Rel).
+
+  Import ltl_prop.
+
+  Lemma ltl_always_introI (P : ltl_prop) :
+     ⊢ P → (□ (P → (○ P))) → □ P.
+  Proof. iIntros "HP HQ". iApply (ltl_always_intro with "HQ HP"). Qed.
+
+  Lemma foo (P Q : ltl_prop) :
+    (P ⊢ ○◊ (P ∧ Q)) → (P ⊢ □◊ Q).
+  Proof.
+    iIntros (HPQ) "HP".
+    iAssert (□ ◊ (P ∧ Q))%I with "[-]" as "[_ $]".
+    iApply (ltl_always_introI with "[HP]").
+    { iDestruct (HPQ with "HP") as "HP".
+      by rewrite ltl_next_eventually. }
+    iIntros "!> [HP _]".
+    rewrite -ltl_eventually_next_comm.
+    iModEv with "HP".
+    rewrite ltl_eventually_next_comm. by iApply HPQ.
+  Qed.
+
+  Lemma bar (P Q : ltl_prop) :
+    □ P ∧ ◊ (P → ○ ◊ Q) ⊢ ◊ Q.
+  Proof.
+    iIntros "[HP HPQ]". iCombine "HPQ HP" as "HPQ".
+    iModEv with "HPQ" as "[HPQ >HP]".
+    iApply ltl_next_eventually.
+    by iApply ("HPQ" with "HP").
+  Qed.
+
+  Lemma baz (P Q : ltl_prop) :
+    (□ (P ∧ Q)) ∧ ○ P ∧ Q ⊢ □ Q.
+  Proof. iIntros "[[HP HQ] [HP' HQ']]". iIntros "!>". by iMod "HQ". Qed.
+
+  Lemma running_example (P : ltl_prop) :
+    □ (P → ○○P) ∧ P ⊢ □ ◊ P.
+  Proof.
+    iIntros "[HP1 HP2]".
+    iAssert (□ (P ∨ (○P)))%I with "[HP1 HP2]" as "H".
+    { iApply (ltl_always_introI with "[HP2]").
+      { by iLeft. }
+      iIntros "!> [HP|HP]".
+      + rewrite ltl_always_elim. iDestruct ("HP1" with "HP") as "HP".
+        iIntros "!>". by iRight.
+      + iIntros "!>". by iLeft. }
+    iIntros "!>".
+    rewrite ltl_always_elim.
+    iDestruct "H" as "[H|H]".
+    - by iApply ltl_eventually_intro_now.
+    - iApply ltl_next_eventually.
+      iIntros "!>".
+      by iApply ltl_eventually_intro_now.
+  Qed.
+
+  Lemma ltl_always_eventually_intro (P : ltl_prop) :
+    □ (P → ○◊ P) ∧ P ⊢ □ ◊ P.
+  Proof.
+    iIntros "[HP1 HP2]".
+    iApply (ltl_always_introI with "[HP2]").
+    { by iApply ltl_eventually_intro_now. }
+    iIntros "!> HP". iApply ltl_eventually_next_comm.
+    iCombine "HP" "HP1" as "HP".
+    iModEv with "HP" as "[HP >HP1]".
+    iDestruct ("HP1" with "HP") as "HP".
+    by iApply ltl_eventually_next_comm.
+  Qed.
+
+  Lemma running_example_alt (P : ltl_prop) :
+    □ (P → ○○P) ∧ P ⊢ □ ◊ P.
+  Proof.
+    iIntros "[HP1 HP2]".
+    iApply ltl_always_eventually_intro. iFrame.
+    iIntros "!> HP". rewrite ltl_always_elim.
+    iDestruct ("HP1" with "HP") as "HP".
+    iIntros "!>".
+    iApply ltl_eventually_intro_next.
+    done.
+  Qed.
+
+  Lemma ltl_until_example (P Q : ltl_prop) :
+    P ∪ Q ∧ (¬ □ P) ⊢ ◊ Q.
+  Proof. rewrite -ltl_until_eventually. apply bi.and_elim_l. Qed.
+
+  (* Lemma foo' {X} (P Q R : X → ltl_prop) : *)
+  (*   ○ (∃ x, P x) ∧ □ ○ ∀ x, (P x → □ Q x) ∧ ◊ ○ ∀ x, (Q x  → R x) ⊢ ∀ x, ○ ◊ R x. *)
+  (* Proof. *)
+  (*   iIntros "(HP & HPQ & HQR)". iIntros "!>". *)
+  (*   iMod "HPQ". iDestruct ("HPQ" with "HP") as "HQ". *)
+  (*   iCombine "HQR" "HQ" as "H". iModEv with "H" as "[HQR HQ]". *)
+  (*   iApply ltl_eventually_intro. iApply "HQR". by iMod "HQ". *)
+  (* Qed. *)
+
+  Lemma bar' (P Q R : Prop) : 
+    P ∧ (P -> Q) -> Q.
+  Proof.
+    intros [HP HPQ].
+    apply HPQ.
+    apply HP.
+  Qed.
+
+  Lemma bar'' (P Q R : ltl_prop) : 
+    P ∧ (P → ◊ Q) ⊢ ◊ Q.
+  Proof.
+    iIntros "[HP HPQ]".
+    iDestruct ("HPQ" with "HP") as "HQ".
+    iApply "HQ".
+  Qed.  
+
+  Lemma foo' (P Q R : ltl_prop) :
+    ○ P ∧ □ ○ (P → □ Q) ∧ ◊ ○ (Q → R) ⊢ ○ ◊ R.
+  Proof.
+    iIntros "(HP & HPQ & HQR)".
+    iModIntro.
+    iMod "HPQ". iDestruct ("HPQ" with "HP") as "HQ".
+    iCombine "HQR" "HQ" as "H". iModEv with "H" as "[HQR HQ]".
+    iApply ltl_eventually_intro_now. iApply "HQR". by iMod "HQ".
+  Qed.
+
+  Lemma foo'' (P Q R : nat → ltl_prop) :
+    ○ (∃ n, P n) ∧ □ ○ (∀ n, P n → ∃ m, □ Q m) ∧
+    ◊ ○ (∀ m, Q m → ∃ k, R k) ⊢ ○ ◊ ∃ k, R k.
+  Proof.
+    iIntros "(HP & HPQ & HQR)".
+    iModIntro. iDestruct "HP" as (n) "HP".
+    iMod "HPQ". iDestruct ("HPQ" with "HP") as (m) "HQ".
+    iCombine "HQR" "HQ" as "H". iModEv with "H" as "[HQR HQ]".
+    iApply ltl_eventually_intro_now. iApply "HQR". by iMod "HQ".
+  Qed.
+
+End examples.
+
+Notation "↓s Φ" := (↓ (λ osl, match osl with
+                              | Some (s,l) => Φ (Some s)
+                              | None => Φ None
+                              end))%I (at level 20, right associativity) : bi_scope. 
+
+Notation "↓l Φ" := (↓ (λ osl, match osl with
+                              | Some (s,Some l) => Φ (Some l)
+                              | Some (s,None) => Φ None
+                              | None => Φ None
+                              end))%I (at level 20, right associativity) : bi_scope. 
+
+Section simple_ex.
+  Definition state := nat.
+  Definition label := unit.
+  Inductive steps : state → label → state → Prop :=
+    | my_step i : steps i () (i+1).
+
+  (* TODO: Why is this needed for [unseal]? *)
+  Import ltl_prop.
+
+  Inductive empty : SProp := .
+
+  Instance steps_dec s oζ c' : Decision (steps s oζ c').
+  Proof.
+    destruct (decide (c' = s + 1)).
+    - subst. constructor 1. destruct oζ. constructor.
+    - constructor 2. intros H. inversion H. subst. done.
+  Qed.
+  
+  Lemma step i :
+    (↓s (λ os, os = Some i)) ⊢
+    (○ (↓s (λ os, os = Some (i+1)))):ltl_prop state label steps.
+  Proof.
+    constructor. intros [[tr|]]; last first.
+    { rewrite ltl_now_unseal.
+      intros H. inversion H; simplify_eq. }
+    rewrite ltl_now_unseal.
+    intros H.
+    destruct tr; inversion H; simplify_eq.
+    - assert ((∀ oζ c', ¬ steps s oζ c')) as Hwf.
+      { intros.
+        destruct (decide (steps s oζ c')); [|done].
+        apply empty_ind. inversion tr_wf. subst. specialize (H2 oζ c'). done. }
+      inversion H0; simplify_eq.
+      specialize (Hwf () (i+1)).
+      pose proof (my_step i). done.
+    - simpl in *. simplify_eq.  
+      assert (∃ oζ c', head_trace (Some tr') = Some c' ∧ steps i oζ c') as Hwf.
+      { destruct tr'.
+        { exfalso. apply empty_ind. inversion tr_wf. simplify_eq. inversion H5.
+          subst.
+          specialize (H1 () (s+1)). 
+          assert (steps s () (s+1)).
+          { constructor. }
+          done. } 
+        exists ℓ, s. split; [done|].
+        destruct (decide (steps i ℓ s)); [done|].
+        exfalso. apply empty_ind. inversion tr_wf. simplify_eq.
+        simpl in *. simplify_eq. destruct l. destruct ℓ. done. }
+      destruct Hwf as (l'&i'&Htr&Hsteps).
+      inversion Hsteps. simplify_eq.
+      (* TODO: Merge *)
+      simpl in *. destruct tr'; simplify_eq.
+      { rewrite ltl_next_unseal. econstructor. econstructor 2; done. }
+      simpl in *.
+      rewrite ltl_next_unseal. econstructor. econstructor 3; done. 
+      Unshelve.
+      { inversion tr_wf. simplify_eq. done. }
+      { inversion tr_wf. simplify_eq. done. }
+  Qed.
+
+  Lemma my_property (n:nat) : 
+    ↓s (λ os, os = Some 0) ⊢ (◊ ↓s (λ os, os = Some n)):ltl_prop nat unit steps.
+  Proof.
+    assert (∃ i j, i = 0 ∧ n-j = i ∧ n >= j) as (i&j&<-&H1&H2).
+    { eexists _, n. split; [done|]. lia. } 
+    revert n i H1 H2. induction j; intros n i H1 H2.
+    { simplify_eq. rewrite right_id. iApply ltl_eventually_intro_now. }
+    iIntros "H".
+    iDestruct (step with "H") as "H".
+    iApply ltl_next_eventually. iModIntro.
+    iDestruct (IHj with "H") as "H".
+    { instantiate (1:=n). rewrite -H1. lia. }
+    { lia. }
+    done.
+  Qed.
+
+End simple_ex.
+
+Section advanced_ex.
+
+  Definition state' : Set := nat * bool.
+  Definition label' : Set := bool.
+  Inductive steps' : state' → label' → state' → Prop :=
+  | my_step_succ i b : steps' (i,b) b (i+1,negb b)
+  | my_step_fail i b : steps' (i,b) (negb b) (i,b).
+
+  Axiom fair :
+    ∀ (b:bool), ⊢ (◊ (↓l (λ ol, ol = Some b))):ltl_prop state' label'.
+
+  (* TODO: Why is this needed for [unseal]? *)
+  Import ltl_prop.
+
+  Lemma step_b b i :
+    (well_formed_trace steps') ∧
+    (↓s (λ os, os = Some (i,b))) ⊢
+         ((↓l (λ ol, ol = Some b)) ∧ ○ (↓s (λ os, os = Some (i+1,negb b)))) ∨
+           ((↓l (λ ol, ol = Some (negb b)) ∧ ○ (↓s (λ os, os = Some (i,b))))).
+  Proof.
+    constructor. intros [tr|]; last first.
+    { unseal. rewrite ltl_now_unseal.
+      intros [_ H]. inversion H. simplify_eq. }
+    unseal. rewrite ltl_now_unseal.
+    intros [Hwf H]. inversion H; simplify_eq.
+    - rewrite /well_formed_trace in Hwf. rewrite ltl_always_unseal in Hwf.
+      inversion Hwf. simplify_eq.
+      inversion H1. simplify_eq.
+      specialize (H3 b ((i+1), negb b)).
+      pose proof (my_step_succ i b). done.
+    - rewrite /well_formed_trace in Hwf. rewrite ltl_always_unseal in Hwf.
+      inversion Hwf. simplify_eq. inversion H2.
+      (* TODO: Merge *)
+      simpl in *. rewrite ltl_next_unseal.
+      destruct tr0; simplify_eq.
+      { inversion H6; simplify_eq.
+        - constructor 1. 
+          constructor.
+          + by constructor.
+          + constructor. constructor. done.
+        - constructor 2.
+          constructor.
+          + constructor. done.
+          + constructor. constructor. done. }
+      { inversion H6; simplify_eq.
+        - constructor 1.
+          constructor.
+          + by constructor.
+          + constructor. constructor. done.
+        - constructor 2.
+          constructor.
+          + constructor. done.
+          + constructor. constructor. done. }
+  Qed.
+
+  Lemma my_property'' i b :
+    (well_formed_trace steps') ∧
+    ↓s (λ os, os = Some (i,b)) ⊢
+    ↓s (λ os, os = Some (i,b)) ∪ ↓s (λ os, os = Some (i+1,negb b)) : ltl_prop state' label'.
+  Proof.
+    iIntros "H".
+    iDestruct (fair b) as "H1".
+    iRevert "H".
+    iApply (ltl_until_ind with "H1").
+    { iIntros "H1 H2".
+       iDestruct (step_b with "H2") as "#[H3|H3]"; last first.
+       { iDestruct "H3" as "[H3 H3']".
+         iDestruct (ltl_now_false with "H1 H3") as "[]".
+         destruct b; intros [[? []]|] HP HQ; by naive_solver. }
+       iDestruct "H3" as "[_ H3']".
+       iApply ltl_until_intro_next. iDestruct "H2" as "[_ H]". iFrame.
+       iModIntro. iApply ltl_until_intro_now. done. }
+    iIntros "[H1 [H2 _]] #H3".
+    iDestruct (step_b with "H3") as "-#[H3'|H3']".
+    { iApply ltl_until_intro_next.
+      iDestruct "H3" as "(Hwf&H3)".
+      iFrame "#".
+      iDestruct "H3'" as "[H' H'']".
+      iModIntro.
+      iApply ltl_until_intro_now.
+      iApply (ltl_now_mono with "H''"). done. }
+    iDestruct "H3'" as "[H' H'']".
+    iDestruct "H3" as "(Hwf&H3)".
+    iApply ltl_until_intro_next.
+    iFrame "#".
+    iModIntro.
+    iApply "H2".
+    iFrame "#".
+    done.
+  Qed.
+
+  Lemma ltl_until_ind_alt {S L} (P P' Q R : ltl_prop S L) :
+    (□ P' ∧ Q ⊢ R) →
+    (□ P' ∧ ○ (ltl_until P Q) ∧ ○ R ∧ P ⊢ R) →
+    □ P' ∧ P ∪ Q ⊢ R.
+  Proof.
+    intros H1 H2. rewrite ltl_until_always_combine.
+    apply ltl_until_ind.
+    - done.
+    - iIntros "(H1 & H2 & H3 & H4)". iApply H2. 
+      iFrame. iModIntro. iApply (ltl_until_mono with "H1"); iIntros "[_ $]".
+  Qed.
+
+  (* Tactic Notation "iIndUntil" "with" constr(pat) := *)
+  (*   iApply (ltl_until_ind with pat); *)
+  (*   [iIntros pat|iIntros "(?&?&?)"]. *)
+
+  (* Tactic Notation "iIndUntil" "with" constr(pat1) "and" constr(pat2) := *)
+  (*   iCombine  *)
+  (*   iApply (ltl_until_ind_alt with pat). *)
+
+  Lemma my_property' n b :
+    (well_formed_trace steps') ∧
+    ↓s (λ os, os = Some (0,b)) ⊢ ∃ b, (◊ ↓s (λ os, os = Some (n,b))):ltl_prop state' label'.
+  Proof.
+    assert (∃ i j, i = 0 ∧ n-j = i ∧ n >= j) as (i&j&<-&H1&H2).
+    { eexists _, n. split; [done|]. lia. } 
+    revert n i b H1 H2. induction j; intros n i b H1 H2.
+    { simplify_eq. rewrite right_id. iIntros "[_ H]". iExists b. iApply ltl_eventually_intro_now. done. }
+    iIntros "#H".
+    iDestruct (my_property'' with "H") as "H'".
+    iDestruct "H" as "(#Hwf & H)".
+    iCombine "H'" "Hwf" as "H''".
+    iApply (ltl_until_ind with "H''").
+    { iIntros "H".
+      iDestruct (IHj with "H") as "H".
+      { instantiate (1:=n). rewrite -H1. lia. }
+      { lia. }
+      done. }
+    iIntros "(H1&H2&H3)".
+    clear IHj.
+    rewrite ltl_next_exists.
+    iDestruct "H2" as (b') "H2".
+    iExists b'.
+    iApply ltl_next_eventually. iModIntro.
+    done.
+  Qed.
+
+End advanced_ex.
